Started section on heap operations.

src/SLImp/ILImp.v
@@ -694,29 +694,29 @@ Proof.
     assumption.
 Qed. 
 
-Fixpoint modified_by (c : com) (l : list id) : list id :=
+Fixpoint modified_by (c : com) : list id :=
   match c with
-  | SKIP => l
-  | i ::= _ => i :: l
-  | c1; c2 =>  modified_by c2 l ++ modified_by c2 l ++ l 
-  | IFB _ THEN c1 ELSE c2 FI => modified_by c1 l ++ (modified_by c2 l ++ l)
-  | WHILE _ DO c END => modified_by c l ++ l
-  | i &= ALLOC _ => i :: l
-  | DEALLOC _ => l
-  | i <~ [ _ ] => i :: l
-  | [ _ ] <~ _ => l
+  | SKIP => nil
+  | i ::= _ => i :: nil
+  | c1; c2 =>  modified_by c1 ++ modified_by c2
+  | IFB _ THEN c1 ELSE c2 FI => modified_by c1 ++ modified_by c2
+  | WHILE _ DO c END => modified_by c
+  | i &= ALLOC _ => i :: nil
+  | DEALLOC _ => nil
+  | i <~ [ _ ] => i :: nil
+  | [ _ ] <~ _ => nil
   end.
   
-Fixpoint list_sub (vs : list id) (l : list id) (ost : state) (ast : state) : state :=
+Fixpoint list_sub (vs : list nat) (l : list id) (ost : state) (ast : state) : state :=
   match vs with
   | vsh :: vs =>
     match l with
-      | lh :: l => list_sub vs l ost (substitute ast ost (cons (vsh, ANum(ost lh)) nil))
-      | _ => ast
+      | lh :: l => list_sub vs l ost (substitute ast ost (cons (lh, ANum(vsh)) nil))
+      | _ => ast (* Lists don't match, should fail instead *)
     end
   | _ =>
     match l with
-      | h :: t => ast
+      | h :: t => ast (* Lists don't match, should fail instead *)
       | _ => ast
     end
   end. 
@@ -731,18 +731,55 @@ Next Obligation.
   apply H0.
 Qed.
         
+Lemma conj_comp : forall (P Q : Assertion) (a b c : Heap) s,
+  P a s ->
+  Q b s ->
+  sa_mul a b c ->
+  (P ** Q) c s.
+Proof.
+  intros.
+  simpl.
+  exists a.
+  exists b.
+  simpl in H1.
+  split.
+    intros k.
+    specialize (H1 k).
+    destruct (find k c).
+    assumption.
+    
+    assumption.
+  
+  split; assumption.
+Qed.
+     
 Theorem frame_rule : forall P Q R c,
-  {{ P }} c {{ Q }} |--
-  {{ P ** R }} c {{ Q ** (Exists vs, var_sub R vs (modified_by c nil)) }}. 
+  {{ P }} c {{ Q }} ->
+  {{ P ** R }} c {{ Q ** (Exists vs, var_sub R vs (modified_by c)) }}. 
 Proof. 
   unfold hoare_triple.
   intros.
   split.
+  Case "safety".
+    
+    
+    
+    
     apply H.
+    inversion H0.
+    inversion H1.
+    inversion H2.
+    simpl in H3.
+    inversion H3.
+      
     
     
+    unfold safe, not.
+    intros.
+    inversion H1; subst.
+    apply H3.
     
-  
+    
 Qed.
 
 Program Definition alloc_cell a : Assertion :=
