report/coq/hoare_example.v
@@ -1,0 +1,2 @@
+Theorem hoare_asgn : forall Q X a,
+  {{assn_sub X a Q}} (X ::= a) {{Q}}.
