report/coq/imp.v
@@ -1,0 +1,27 @@
+Inductive ceval : com -> state -> state -> Prop :=
+  | E_Skip : forall st,
+      SKIP / st || st
+  | E_Ass  : forall st a1 n X,
+      aeval st a1 = n ->
+      (X ::= a1) / st || (update st X n)
+  | E_Seq : forall c1 c2 st st' st'',
+      c1 / st  || st' ->
+      c2 / st' || st'' ->
+      (c1 ; c2) / st || st''
+  | E_IfTrue : forall st st' b1 c1 c2,
+      beval st b1 = true ->
+      c1 / st || st' ->
+      (IFB b1 THEN c1 ELSE c2 FI) / st || st'
+  | E_IfFalse : forall st st' b1 c1 c2,
+      beval st b1 = false ->
+      c2 / st || st' ->
+      (IFB b1 THEN c1 ELSE c2 FI) / st || st'
+  | E_WhileEnd : forall b1 st c1,
+      beval st b1 = false ->
+      (WHILE b1 DO c1 END) / st || st
+  | E_WhileLoop : forall st st' st'' b1 c1,
+      beval st b1 = true ->
+      c1 / st || st' ->
+      (WHILE b1 DO c1 END) / st' || st'' ->
+      (WHILE b1 DO c1 END) / st || st''   
+  where "c1 '/' st '||' st'" := (ceval c1 st st').
